Add assertion subtypes
Add location_assertion type
Add top_assertion type
Add location_invariant type
Add top_invariant type
Add self_invariant type

tlc/syntax/assertion.v
@@ -1,6 +1,8 @@
 Require Import mathcomp.ssreflect.eqtype.
+Require Import mathcomp.ssreflect.seq.
 Require Import mathcomp.ssreflect.ssrbool.
 Require Import mathcomp.ssreflect.ssreflect.
+Require Import mathcomp.ssreflect.ssrnat.
 Require Import tlc.operation.orientation.
 Require Import tlc.syntax.constructor.
 Require Import tlc.syntax.literal.
@@ -8,6 +10,7 @@ Require Import tlc.syntax.parameter.
 Require Import tlc.syntax.predicate.
 Require Import tlc.syntax.term.
 Require Import tlc.syntax.variable.
+Require Import tlc.utility.seq.
 
 Set Implicit Arguments.
 Unset Strict Implicit.
@@ -122,9 +125,9 @@ Notation "{A: A }" := (A%assertion)
 Notation "# p" := (APredicate p) : assertion_scope.
 Notation "~ A" := (ANot A) : assertion_scope.
 Notation "Al /\ Ar" := (AAnd Al Ar) : assertion_scope.
-Notation "forall: v , A" := (AForAll v A)
-  (at level 65, v at level 99, A at level 200, right associativity)
-  : assertion_scope.
+Notation "forall: v1 , .. , vn : A" := (AForAll v1 (.. (AForAll vn A) ..))
+  (at level 65, v1 at level 99, vn at level 99, A at level 200,
+    right associativity) : assertion_scope.
 Notation "always^ A" := (AAlways' A)
   (at level 60, right associativity) : assertion_scope.
 Notation "alwaysp^ A" := (AAlwaysP' A)
@@ -141,62 +144,62 @@ Notation "'self' A" := (ASelf A)
   (at level 60, right associativity) : assertion_scope.
 
 (* Predicate notations *)
-Definition AFalse := {A: # PFalse}.
-Definition AEqual tl tr := {A: # (PEqual tl tr)}.
+Notation AFalse := {A: # PFalse}.
+Notation AEqual tl tr := {A: # (PEqual tl tr)}.
 Notation "tl = tr" := (AEqual tl tr) : assertion_scope.
-Definition AIn t ts := {A: # (PIn t ts)}.
+Notation AIn t ts := {A: # (PIn t ts)}.
 Notation "t \in ts" := (AIn t ts) : assertion_scope.
-Definition AExtension ts' ts := {A: # (PExtension ts' ts)}.
+Notation AExtension ts' ts := {A: # (PExtension ts' ts)}.
 Notation "ts' <<< ts" := (AExtension ts' ts)
   (at level 20, no associativity) : assertion_scope.
-Definition ACorrect tn := {A: # (PCorrect tn)}.
+Notation ACorrect tn := {A: # (PCorrect tn)}.
 Notation "'correct' tn" := (ACorrect tn)
   (at level 0, no associativity) : assertion_scope.
 
 (* Derived propositional operators *)
-Definition AOr Al Ar := {A: ~(~Al /\ ~Ar)}.
+Notation AOr Al Ar := {A: ~(~Al /\ ~Ar)}.
 Notation "Al \/ Ar" := (AOr Al Ar) : assertion_scope.
-Definition AIf Al Ar := {A: ~Al \/ Ar}.
+Notation AIf Al Ar := {A: ~Al \/ Ar}.
 Notation "Al -> Ar" := (AIf Al Ar) : assertion_scope.
-Definition AIff Al Ar := {A: (Al -> Ar) /\ (Ar -> Al)}.
+Notation AIff Al Ar := {A: (Al -> Ar) /\ (Ar -> Al)}.
 Notation "Al <-> Ar" := (AIff Al Ar) : assertion_scope.
-Definition AExists v A := {A: ~forall: v, ~A}.
-Notation "exists: v , A" := (AExists v A)
+Notation AExists v A := {A: ~forall: v: ~A}.
+Notation "exists: v : A" := (AExists v A)
   (at level 65, v at level 99, A at level 200, right associativity)
   : assertion_scope.
 
 (* Derived strict and immediate past temporal operators *)
-Definition APrevious' A := {A: ~previous ~A}.
+Notation APrevious' A := {A: ~previous ~A}.
 Notation "previous^ A" := (APrevious' A)
   (at level 60, right associativity) : assertion_scope.
 
 (* Derived reflexive future temporal operators *)
-Definition AEventually A := {A: A \/ eventually^ A}.
+Notation AEventually A := {A: A \/ eventually^ A}.
 Notation "'eventually' A" := (AEventually A)
   (at level 60, right associativity) : assertion_scope.
-Definition AAlways A := {A: A /\ always^ A}.
+Notation AAlways A := {A: A /\ always^ A}.
 Notation "'always' A" := (AAlways A)
   (at level 60, right associativity) : assertion_scope.
 
 (* Derived reflexive past temporal operators *)
-Definition AEventuallyP A := {A: A \/ eventuallyp^ A}.
+Notation AEventuallyP A := {A: A \/ eventuallyp^ A}.
 Notation "'eventuallyp' A" := (AEventuallyP A)
   (at level 60, right associativity) : assertion_scope.
-Definition AAlwaysP A := {A: A /\ alwaysp^ A}.
+Notation AAlwaysP A := {A: A /\ alwaysp^ A}.
 Notation "'alwaysp' A" := (AAlwaysP A)
   (at level 60, right associativity) : assertion_scope.
 
 (* Additional temporal operators *)
-Definition AEntails Al Ar := {A: always (Al -> Ar)}.
+Notation AEntails Al Ar := {A: always (Al -> Ar)}.
 Notation "Al =>> Ar" := (AEntails Al Ar)
   (at level 99, right associativity) : assertion_scope.
-Definition ACongruent Al Ar := {A: (Al =>> Ar) /\ (Ar =>> Al)}.
+Notation ACongruent Al Ar := {A: (Al =>> Ar) /\ (Ar =>> Al)}.
 Notation "Al <=> Ar" := (ACongruent Al Ar)
   (at level 95, no associativity) : assertion_scope.
-Definition AFollowedBy Al Ar := {A: Al =>> eventually Ar}.
+Notation AFollowedBy Al Ar := {A: Al =>> eventually Ar}.
 Notation "Al ~> Ar" := (AFollowedBy Al Ar)
   (at level 90, right associativity) : assertion_scope.
-Definition APrecededBy Al Ar := {A: Al =>> eventuallyp Ar}.
+Notation APrecededBy Al Ar := {A: Al =>> eventuallyp Ar}.
 Notation "Al <~ Ar" := (APrecededBy Al Ar)
   (at level 90, right associativity) : assertion_scope.
 
@@ -229,7 +232,7 @@ Definition AWhenSubPeriodic ti te :=
 Notation "when[ ti ]~> te" := (AWhenSubPeriodic ti te)
   (at level 60, no associativity) : assertion_scope.
 Definition AWhenSelf :=
-  {A: (exists: "i", "Fd" = ["i"] /\ "Fo" = OIndication) \/
+  {A: (exists: "i": "Fd" = ["i"] /\ "Fo" = OIndication) \/
     ("Fd" = [] /\ "Fo" = ORequest) \/
     ("Fd" = [] /\ "Fo" = OPeriodic)}.
 Notation "when-self" := (AWhenSelf)
@@ -255,7 +258,104 @@ Inductive non_temporal_assertion : assertion -> Type :=
   non_temporal_assertion {A: Al /\ Ar}
 | NTAForAll v A :
   non_temporal_assertion A ->
-  non_temporal_assertion {A: forall: v, A}.
+  non_temporal_assertion {A: forall: v: A}.
 
 Definition non_temporal_assertion_t :=
   {A : assertion & non_temporal_assertion A}.
+
+(* Proposition for assertions at a particular location *)
+Inductive location_assertion : seq nat -> assertion -> Type :=
+| LAEventOn d tn d' to te :
+  extension d' d ->
+  location_assertion d {A: when-on[tn]
+    ("Fd" = (TList [seq TLiteral (LNatural i) | i <- d']) /\
+      "Fo" = to /\ "Fe" = te)}
+| LACorrect d tn :
+  location_assertion d {A: correct tn}
+| LANot d A :
+  location_assertion d A ->
+  location_assertion d {A: ~A}
+| LAAnd d Al Ar :
+  location_assertion d Al ->
+  location_assertion d Ar ->
+  location_assertion d {A: Al /\ Ar}
+| LAForAll d v A :
+  location_assertion d A ->
+  location_assertion d {A: forall: v: A}
+| LAAlways' d A :
+  location_assertion d A ->
+  location_assertion d {A: always^ A}
+| LAAlwaysP' d A :
+  location_assertion d A ->
+  location_assertion d {A: alwaysp^ A}
+| LAEventually' d A :
+  location_assertion d A ->
+  location_assertion d {A: eventually^ A}
+| LAEventuallyP' d A :
+  location_assertion d A ->
+  location_assertion d {A: eventuallyp^ A}.
+
+Definition local_assertion_t d :=
+  {A : assertion & location_assertion d A}.
+
+(* Proposition for assertions on the top component *)
+Definition top_assertion := location_assertion [::].
+
+Definition top_assertion_t :=
+  {A : assertion & top_assertion A}.
+
+(* Proposition for assertions that are invariants at a particular location *)
+Inductive location_invariant : seq nat -> assertion -> Type :=
+| LIA d A:
+  location_assertion d {A: always A} ->
+  location_invariant d A.
+
+Definition location_invariant_t d :=
+  {A : assertion & location_invariant d A}.
+
+Lemma location_invariant_assertion d A :
+  location_invariant d A ->
+  location_assertion d {A: always A}.
+Proof.
+  move=> LI.
+  by inversion LI; subst.
+Qed.
+
+(* Proposition for assertions that are invariants on the top component *)
+Definition top_invariant := location_invariant [::].
+
+Definition top_invariant_t :=
+  {A : assertion & top_invariant A}.
+
+(* Proposition for assertions that are self invariants *)
+Inductive self_invariant : assertion -> Type :=
+| SITopRequestOn tn te :
+  self_invariant {A: when-on[tn] when[]-> te}
+| SITopPeriodicOn tn te :
+  self_invariant {A: when-on[tn] when[]~> te}
+| SISubIndicationOn tn ti te :
+  self_invariant {A: when-on[tn] when[ti]<- te}
+| SICorrect tn :
+  self_invariant {A: correct tn}
+| SINot A :
+  self_invariant A ->
+  self_invariant {A: ~A}
+| SIAnd Al Ar :
+  self_invariant Al ->
+  self_invariant Ar ->
+  self_invariant {A: Al /\ Ar}
+| SIForAll v A :
+  self_invariant A ->
+  self_invariant {A: forall: v: A}
+| SIAlways' A :
+  self_invariant A ->
+  self_invariant {A: always^ A}
+| SIAlwaysP' A :
+  self_invariant A ->
+  self_invariant {A: alwaysp^ A}
+| SIEventually' A :
+  self_invariant A ->
+  self_invariant {A: eventually^ A}
+| SIEventuallyP' A :
+  self_invariant A ->
+  self_invariant {A: eventuallyp^ A}.
